\subsection{Left Factoring \& Left Recursion}

\subsubsection{Left Factoring Productions}

\subsubsubsection{Left Factor Rewriting Rule}
To remove the left factor from
\begin{align*}
    A \rightarrow \alpha\ \beta\ |\ \alpha\ \gamma,
\end{align*}
we can rewrite the production using an aditional nonterminal $A'$ as
\begin{equation*}
    \begin{aligned}[c]
        A &\rightarrow \alpha\ A'
    \end{aligned}
    \qquad 
    \begin{aligned}[c]
        A' &\rightarrow \beta\ |\ \gamma
    \end{aligned}
\end{equation*}
\subsubsection{Left Recursive Productions}
\subsubsubsection{Immediate Left Recursion Rewriting Rule (Simple)}
To remove the left recursion from
\begin{align*}
    A \rightarrow A\ \alpha\ |\ \beta,
\end{align*}
we can rewrite the production as
\begin{equation*}
    \begin{aligned}[c]
        A &\rightarrow \beta\ A'
    \end{aligned}
    \qquad 
    \begin{aligned}[c]
        A' &\rightarrow \epsilon\ |\ \alpha\ A'
    \end{aligned}
\end{equation*}

\subsubsubsection{Immediate Left Recursion Rewriting Rule (General)}
To remove the left recursion from the general case
\begin{align*}
    A \rightarrow A\alpha_1|A\alpha_2|\dots|A\alpha_n|\beta_1|\beta_2|\dots|\beta_m,
\end{align*}
we can use grouping to see the structure in the same form as the simple case
\begin{align*}
    A \rightarrow A(\alpha_1|\alpha_2|\dots|\alpha_n)|(\beta_1|\beta_2|\dots|\beta_m)
\end{align*}
which allows us to rewrite the production as follows,
\begin{align*}
    A &\rightarrow (\beta_1|\beta_2|\dots|\beta_m)A'\\
    A' &\rightarrow \epsilon|(\alpha_1|\alpha_2|\dots|\alpha_n)A'
\end{align*}

\subsubsubsection{Indirect Left Recursion Rewriting Rule}
The following productions have indirect recursion from $A \rightarrow B \rightarrow C \rightarrow A$.
\begin{equation*}
    \begin{aligned}[c]
        A &\rightarrow B\ \alpha
    \end{aligned}
    \quad 
    \begin{aligned}[c]
        B &\rightarrow C\ \beta
    \end{aligned}
    \quad
    \begin{aligned}[c]
        C &\rightarrow A\ \gamma_1\ |\  \gamma_2
    \end{aligned}
\end{equation*}

To remove the recursion we can first collapse $B$ into $A$ as follows.
\begin{equation*}
    \begin{aligned}[c]
        A &\rightarrow C\ \beta\ \alpha
    \end{aligned}
    \qquad 
    \begin{aligned}[c]
        C &\rightarrow A\ \gamma_1\ |\ \gamma_2
    \end{aligned}
\end{equation*}
Then we can collapse $C$ into $A$.
\begin{align*}
    A &\rightarrow (A\ \gamma_1\ |\  \gamma_2)\ \beta\ \alpha\\
    &\ \ \ \ \ \ \ \ \ \ \downarrow\\
    A &\rightarrow A\ \gamma_1\ \beta\ \alpha\ |\ \gamma_2\ \beta\ \alpha
\end{align*}
This now leaves a simple direct left recursion which we can remove as follows.
\begin{equation*}
    \begin{aligned}[c]
        A &\rightarrow \gamma_2\ \beta\ \alpha\ A'\\
    \end{aligned}
    \qquad 
    \begin{aligned}[c]
        A' &\rightarrow \gamma_1\ \beta\ \alpha\ A'
    \end{aligned}
\end{equation*}