\section{Question 1}

\subsection{Predicate Logic}

\begin{tabular}{@{}ll@{}}
\fontsize{5pt}{6pt}\selectfont
$ A \land (A \lor B) \equiv A \equiv A \lor (A \land B)$ & \verb! (A.6)! \\
$ A \land (B \lor C) \equiv (A \land B) \lor (A \land C)$ & \verb! (A.7)! \\
$ A \lor (B \land C) \equiv (A \lor B) \land (A \lor C)$ & \verb! (A.8)! \\
$ \neg (A \land B) \equiv \neg A \lor \neg B$ & \verb! (A.18)! \\
$ \neg (A \lor B) \equiv \neg A \land \neg B$ & \verb! (A.19)! \\
$ A \lor (\neg A \land B) \equiv A \lor B$ & \verb! (A.20)! \\
$ A \land (\neg A \lor B) \equiv A \land B$ & \verb! (A.21)! \\
$ A \imp B \equiv \neg A \lor B$ & \verb! (A.22)! \\
$ A \imp B \equiv \neg(A \land \neg B)$ & \verb! (A.24)! \\
$ \neg(A \imp B) \equiv A \land \neg B$ & \verb! (A.25)! \\
$ A \imp B \equiv \neg B \imp \neg A$ & \verb! (A.26)! \\
$ C \imp (A \land B) \equiv (C \imp A) \land (C \imp B)$ & \verb! (A.33)! \\
$ (A \lor B) \imp C \equiv (A \imp C) \land (B \imp C)$ & \verb! (A.34)! \\
$ C \imp (A \lor B) \equiv (C \imp A) \lor (C \imp B)$ & \verb! (A.35)! \\
$ (A \land B) \imp C \equiv (A \imp C) \lor (B \imp C)$ & \verb! (A.36)! \\
$ A \imp (B \imp C) \equiv (A \land B) \imp C \equiv$ & \verb! (A.37)! \\
$ B \imp (A \imp C)$ & \\
$ (A \imp B) \land (\neg A \imp C) \equiv$ & \verb! (A.38)! \\
$ (A \land B) \lor (\neg A \land C)$ & \\
$ (\forall x \text{ s.t. } x = E \imp A) \equiv A[x \backslash E] \equiv $ & \verb! (A.56)! \\
$ (\exists x \text{ s.t. } x = E \land A)$ & \\
$ \forall x :: A \land B = (\forall x :: A) \land (\forall x :: B)$ & \verb! (A.65)! \\
$ \forall x :: A = A \text{ provided } x \text{ not free in } A$ & \verb! (A.74)! \\
\end{tabular}

\subsection{Rules to know}

\subsubsection{Basic Function} 
\begin{verbatim}
method MyMethod(x: int) returns (y: int)
    requires x == 10
    ensures y >= 25
{
    {x == 10}
    {x + 3 + 12 == 25}
    var a := x + 3;
    {a + 12 == 25}
    var b := 12;
    {a + b == 25}
    y := a + b;
    {y >= 25}
}

\end{verbatim}


\subsubsection{Loops} 
\begin{verbatim}
{J}
while B
        invariant J
{
        {B && J}
        ... 
        {J}
}
{J && !B}
\end{verbatim}

\begin{verbatim}
{y >= 4 && z >= x}
while z < 0
        invariant y >= 4 && z >= x
{
        {z < 0 && y >= 4 && z >= x}
        {y >= 4 && z + y >= x}
        z := z + y;
        {y >= 4 && z >= x}
}
{z >= 0 && y >= 4 && z >= x}
\end{verbatim}

\subsubsection{Arrays} 
\begin{verbatim}
var a := new string[20];
# Type of a is array<string>
var m := new bool[3, 10];
# Type of m is array2<bool>

\end{verbatim}
\begin{verbatim}
method LinearSearch<T>(a: array<T>, P: T -> bool)
returns (n: int)
ensures 0 <= n <= a.Length
ensures n == a.Length || P(a[n])
ensures n == a.Length ==>
forall i :: 0 <= i < a.Length ==> !P(a[i])
{
n := 0;
while n != a.Length
        invariant 0 <= n <= a.Length
        invariant forall i :: 0 <= i < n ==>
                        !P(a[i])
{ 0 <= n < a.Length &&
(!P(a[n]) ==> (forall i :: 0 <= i < n ==>
                        !P(a[i])) 
                                && !P(a[n])) }
{ (P(a[n]) ==> 0 <= n <= a.Length &&
(n == a.Length || P(a[n])) &&
(n == a.Length ==>
forall i :: 0 <= i < a.Length ==> !P(a[i]))) &&
(!P(a[n]) ==> (forall i :: 0 <= i < n ==> 
                        !P(a[i])) && !P(a[n])) }
if (P(a[n])) {
        return;
}
{ (forall i :: 0 <= i < n ==> !P(a[i])) (A.56)
&& (forall i :: i == n ==> !P(a[i])) } (A.65)
{ forall i :: (0 <= i < n ==> !P(a[i])) &&
                        (i == n ==>
                        !P(a[i])) } (A.34)
{ forall i :: 0 <= i < n || i == n ==> !P(a[i])}
{ forall i :: 0 <= i < n + 1 ==> !P(a[i]) }
n := n + 1;
{ forall i :: 0 <= i < n ==> !P(a[i]) }
\end{verbatim}

\subsubsection{Methods} 
\begin{verbatim}
wp(t := M(E), Q )
  = P[x\E]
    &&  forall y' ::
      R[x,y\E, y'] 
        ==> Q[t\y']
\end{verbatim}
\begin{verbatim}
Given:
method Triple(x: int) returns (y: int)
requires x >= 0
ensures y == 3*x {}


{ u == 15}
{ u + 3 >= 0 &&
        3*(u + 3) == 54 } (A.56)
{ u + 3 >= 0 &&
        forall y' :: y' == 3*(u + 3)
                ==> y' == 54 }
t := Triple(u + 3);
{ t == 54 }

\end{verbatim}
\begin{verbatim}
function SeqSum(s: seq<int>, lo: int, hi: int): int
requires 0 <= lo <= hi <= |s|
decreases hi - lo
{
        if lo == hi then 0 else s[lo] +
            SeqSum(s, lo + 1, hi)
}
\end{verbatim}